proof/old_system/uni/decl_worklist/prop_equiv.v
@@ -170,11 +170,23 @@ Qed.
 Hint Resolve d_wf_wl_wf_env : Hdb_dworklist_equiv.
 
 
-Theorem d_wf_work_apply_cont : forall Ω c A1 w,
-  ⊢ᵈʷ Ω -> d_wf_cont (dwl_to_denv Ω) c -> dwl_to_denv Ω ⊢ A1 -> apply_cont c A1 w ->
+Theorem d_wf_work_apply_cont : forall Ω c A w,
+  ⊢ᵈʷ Ω -> d_wf_cont (dwl_to_denv Ω) c -> dwl_to_denv Ω ⊢ A -> apply_cont c A w ->
   ⊢ᵈʷ dworklist_conswork Ω w.
 Proof.
   intros. induction H2; simpl; auto;
+    dependent destruction H0; auto.
+Qed.
+
+Theorem d_wf_work_apply_cont2 : forall Ω cc A B w,
+  ⊢ᵈʷ Ω -> 
+  d_wf_cont2 (dwl_to_denv Ω) cc -> 
+  dwl_to_denv Ω ⊢ A -> 
+  dwl_to_denv Ω ⊢ B -> 
+  apply_cont2 cc A B w ->
+  ⊢ᵈʷ dworklist_conswork Ω w.
+Proof.
+  intros. induction H3; simpl; auto;
     dependent destruction H0; auto.
 Qed.
 
@@ -279,9 +291,6 @@ Proof with eauto with Hdb_dworklist_equiv typing.
   - _apply_IH_d_wl_red.
     destruct_d_wl_del_red.
     eapply d_wl_del_red__infabs with (B:=typ_intersection B1 B2) (C:=typ_union C1 C2)...
-  - assert (⊢ᵈʷ (work_infabs A (contd_unioninfabs B C cc) ⫤ Ω)) by admit.
-    apply IHd_wl_red in H1.
-    destruct_d_wl_del_red...  
   - econstructor; eauto.
     destruct_wf.
     eapply d_wf_work_apply_cont in H0; eauto.
@@ -420,13 +429,13 @@ Proof with auto with Hdb_dworklist_equiv.
     destruct_wf.
     econstructor.
     eapply IHd_inftapp1...
-    eapply d_wl_red__applycont with (w:=work_inftappunion C1 A2 B c).
+    eapply d_wl_red__apply_cont with (w:=work_inftappunion C1 A2 B c).
     econstructor.
     simpl.
     econstructor. 
     eapply IHd_inftapp2... intuition.
-    eapply d_wl_red__applycont with (w:=work_unioninftapp C1 C2 c).
-    eapply applycont__unioninftapp...
+    eapply d_wl_red__apply_cont with (w:=work_unioninftapp C1 C2 c).
+    eapply apply_cont__unioninftapp...
     econstructor...
 Qed.
 
@@ -446,7 +455,7 @@ Proof with auto with Hdb_dworklist_equiv.
   - econstructor.
     destruct_wf.
     eapply IHd_typing1; eauto.
-    apply d_wl_red__applycont with (w:=work_infabs A (cont_infapp e2 c)); eauto.
+    apply d_wl_red__apply_cont with (w:=work_infabs A (contd_infapp e2 c)); eauto.
     econstructor. simpl.
     apply d_infabs_wft in H0 as Hwft. intuition.
     eapply d_wl_red_infabs_complete; eauto.
@@ -467,7 +476,7 @@ Proof with auto with Hdb_dworklist_equiv.
     apply d_chk_inf_wft in H0.
     econstructor.
     apply IHd_typing; auto...
-    apply d_wl_red__applycont with (w:=(work_inftapp A B c)); eauto.
+    apply d_wl_red__apply_cont with (w:=(work_inftapp A B c)); eauto.
     econstructor.
     simpl.
     eapply d_wl_red_inftapp_complete; eauto.
@@ -510,8 +519,8 @@ Proof with auto with Hdb_dworklist_equiv.
   - destruct_wf. 
     apply d_wl_red__infabsunion.
     eapply d_wl_red_infabs_complete; eauto.
-    eapply d_wl_red__applycont with (w:=(work_unioninfabs (typ_arrow B1 C1)  (typ_arrow B2 C2) c)).
-    apply applycont__unioninfabs.
+    eapply d_wl_red__apply_cont2 with (w:=(work_unioninfabs B1 C1 B2 C2 cc)).
+    apply apply_cont2__unioninfabs.
     simpl. econstructor.
     apply d_infabs_wft in H4. 
     apply IHd_wl_del_red. intuition.
@@ -523,13 +532,15 @@ Proof with auto with Hdb_dworklist_equiv.
   - destruct_wf. eapply d_wl_red_inftapp_complete; eauto.
   - destruct_wf. econstructor. 
     eapply d_wl_red_inftapp_complete; eauto...
-    eapply d_wl_red__applycont with (w:=(work_unioninftapp C1 C2 c))...
+    eapply d_wl_red__apply_cont with (w:=(work_unioninftapp C1 C2 c))...
     econstructor. simpl.
     apply d_inftapp_wft in H4.
     econstructor. intuition.
   - destruct_wf. apply d_wl_red_sub_complete; eauto.
   - destruct_wf. econstructor; eauto.
     apply IHd_wl_del_red. eapply d_wf_work_apply_cont; eauto.
+  - destruct_wf. econstructor; eauto.
+    apply IHd_wl_del_red. eapply d_wf_work_apply_cont2 in H3; eauto.
 Qed.
 
 
